# baseURI: http://purl.org/dpn/services
# imports: http://purl.org/dpn
# prefix: dpns

@prefix dc: <http://purl.org/dc/terms/> .
@prefix dpn: <http://purl.org/dpn#> .
@prefix dpnd: <http://purl.org/dpn/dataset#> .
@prefix dpns: <http://purl.org/dpn/services#> .
@prefix hr: <http://www.wsmo.org/ns/hrests#> .
@prefix j.0: <http://purl.org/dc/elements/1.1/> .
@prefix msm: <http://iserve.kmi.open.ac.uk/ns/msm#> .
@prefix owl: <http://www.w3.org/2002/07/owl#> .
@prefix rdf: <http://www.w3.org/1999/02/22-rdf-syntax-ns#> .
@prefix rdfs: <http://www.w3.org/2000/01/rdf-schema#> .
@prefix wl: <http://www.wsmo.org/ns/wsmo-lite#> .
@prefix xml: <http://www.w3.org/XML/1998/namespace> .
@prefix xsd: <http://www.w3.org/2001/XMLSchema#> .

<http://purl.org/dpn/services>
  rdf:type owl:Ontology ;
  rdfs:comment "This ontology is being developed by CSIRO under the eReefs project for describing data provider services. Populates DPN service descriptions with vocabulary items" ;
  owl:imports <http://purl.org/dpn> ;
  owl:priorVersion <http://purl.org/dpn/services/v0.1> ;
  owl:versionIRI <http://purl.org/dpn/services/v0.6.1> ;
  owl:versionInfo "v 0.6.1 5/8/2015 Jonathan Yu" ;
.
dpns:CSW
  rdf:type owl:Class ;
  rdfs:comment "A profile of the OGC Catalog Servic" ;
  rdfs:label "Catalogue Service for the Web" ;
  rdfs:seeAlso <http://www.opengeospatial.org/standards/csw> ;
  rdfs:subClassOf dpn:MetadataServiceInterface ;
.
dpns:GeoNetwork
  rdf:type owl:Class ;
  rdfs:comment "GeoNetwork is a catalog application to manage spatially referenced resources." ;
  rdfs:label "GeoNetwork service" ;
  rdfs:seeAlso <http://geonetwork-opensource.org/> ;
  rdfs:subClassOf dpn:Service ;
  rdfs:subClassOf [
      rdf:type owl:Restriction ;
      owl:onProperty dpn:implements ;
      owl:someValuesFrom dpns:CSW ;
    ] ;
.
dpns:GeoServer
  rdf:type owl:Class ;
  rdfs:comment "GeoServer is the reference implementation of the Open Geospatial Consortium (OGC) Web Feature Service (WFS) and Web Coverage Service (WCS) standards, as well as a high performance certified compliant Web Map Service (WMS)." ;
  rdfs:label "GeoServer" ;
  rdfs:seeAlso <http://geoserver.org/> ;
  rdfs:subClassOf dpn:Service ;
  rdfs:subClassOf [
      rdf:type owl:Restriction ;
      owl:onProperty dpn:implements ;
      owl:someValuesFrom dpns:WFS ;
    ] ;
.
dpns:HTTP
  rdf:type owl:Class ;
  rdfs:comment "Hypertext Transfer Protocol" ;
  rdfs:label "HTTP Protocol" ;
  rdfs:subClassOf dpn:DataServiceInterface ;
.
dpns:MapServer
  rdf:type owl:Class ;
  rdfs:comment "MapServer is an open source development environment for building spatially-enabled web mapping applications and services. It supports WMS, WFS and WCS" ;
  rdfs:label "MapServer" ;
  rdfs:seeAlso <http://mapserver.org/> ;
  rdfs:subClassOf dpn:Service ;
  rdfs:subClassOf [
      rdf:type owl:Restriction ;
      owl:onProperty dpn:implements ;
      owl:someValuesFrom dpns:WMS ;
    ] ;
.
dpns:NetcdfSubset
  rdf:type owl:Class ;
  rdf:type owl:NamedIndividual ;
  rdfs:comment "A NetCDF subset dataset" ;
  rdfs:label "NetCDF Subset" ;
  rdfs:subClassOf dpn:DataServiceInterface ;
.
dpns:OpenDAP
  rdf:type owl:Class ;
  rdfs:comment "OpenDAP is a data transfer protocol used widely in the earth sciences. It defines standards for structuring data, and its annotation as well as interfaces for accessing data typically through THREDDS servers often in HDF or NetCDF format. It provides functionality to retrieve subsets of data and aggregation functions as part of the API." ;
  rdfs:label "OpenDAP" ;
  rdfs:seeAlso <http://www.opendap.org/> ;
  rdfs:subClassOf dpn:DataServiceInterface ;
.
dpns:PIDService
  rdf:type owl:Class ;
  rdfs:comment "Persistent Identifier Service allows registry and deferencing identifier handles." ;
  rdfs:label "Persistent Identifier Service" ;
  rdfs:seeAlso <https://www.seegrid.csiro.au/wiki/Siss/PIDService> ;
  rdfs:subClassOf dpn:Service ;
  rdfs:subClassOf [
      rdf:type owl:Restriction ;
      owl:onProperty dpn:implements ;
      owl:someValuesFrom dpn:IdentifierService ;
    ] ;
.
dpns:PromsServiceInterface
  rdf:type owl:Class ;
  rdfs:comment "Provenance Management System (PROMS) service interface allows access to the PROMS implementation for retrieval and storage of provenance instance reports and any semantic annotations" ;
  rdfs:label "PROMS Service Interface" ;
  rdfs:seeAlso <https://wiki.csiro.au/display/pms/Home> ;
  rdfs:subClassOf dpn:ProvenanceServiceInterface ;
.
dpns:SISSVocService
  rdf:type owl:Class ;
  rdfs:comment "Spatial Information Services Stack Vocabulary Service (SISSVoc) is a standard interface through which standard vocabularies can be provided to web users" ;
  rdfs:label "SISSVoc Service" ;
  rdfs:seeAlso <https://www.seegrid.csiro.au/wiki/Siss/VocabularyService> ;
  rdfs:subClassOf dpn:Service ;
  rdfs:subClassOf [
      rdf:type owl:Restriction ;
      owl:allValuesFrom dpn:LinkedDataApiOperation ;
      owl:onProperty wl:hasOperation ;
    ] ;
.
dpns:SISSVocServiceInterface
  rdf:type owl:Class ;
  rdfs:comment "SISSVoc Service Interface definition" ;
  rdfs:label "SISSVoc Service Interface" ;
  rdfs:seeAlso <https://www.seegrid.csiro.au/wiki/Siss/SISSvoc30API> ;
  rdfs:subClassOf dpn:VocabularyServiceInterface ;
.
dpns:SOS
  rdf:type owl:Class ;
  rdfs:label "Sensor Observation Service" ;
  rdfs:seeAlso <http://www.opengeospatial.org/standards/sos> ;
  rdfs:subClassOf dpn:DataServiceInterface ;
.
dpns:THREDDS
  rdf:type owl:Class ;
  rdfs:comment "THREDDS is a web server that provides metadata and data access for scientific datasets, using a variety of remote data access protocols, including OpenDAP, WMS and WCS" ;
  rdfs:label "THREDDS Data Server" ;
  rdfs:seeAlso <https://www.unidata.ucar.edu/software/thredds/current/tds/> ;
  rdfs:subClassOf dpn:Service ;
  rdfs:subClassOf [
      rdf:type owl:Restriction ;
      owl:onProperty dpn:implements ;
      owl:someValuesFrom dpns:OpenDAP ;
    ] ;
  rdfs:subClassOf [
      rdf:type owl:Restriction ;
      owl:onProperty dpn:implements ;
      owl:someValuesFrom dpns:WCS ;
    ] ;
  rdfs:subClassOf [
      rdf:type owl:Restriction ;
      owl:onProperty dpn:implements ;
      owl:someValuesFrom dpns:WMS ;
    ] ;
.
dpns:WCS
  rdf:type owl:Class ;
  rdfs:label "Web Coverage Service" ;
  rdfs:seeAlso <http://www.opengeospatial.org/standards/wcs> ;
  rdfs:subClassOf dpn:DataServiceInterface ;
.
dpns:WFS
  rdf:type owl:Class ;
  rdfs:label "Web Feature Service" ;
  rdfs:seeAlso <http://www.opengeospatial.org/standards/wfs> ;
  rdfs:subClassOf dpn:DataServiceInterface ;
.
dpns:WMS
  rdf:type owl:Class ;
  rdfs:label "Web Mapping Service" ;
  rdfs:seeAlso <http://www.opengeospatial.org/standards/wms> ;
  rdfs:subClassOf dpn:DataServiceInterface ;
.
wl:FunctionalClassificationRoot
  rdf:type rdfs:Class ;
  rdfs:subClassOf rdfs:Class ;
.
wl:Service
  rdf:type owl:Class ;
  rdfs:label "WSMO Lite service description" ;
  rdfs:subClassOf owl:Thing ;
.
